Updates

high2/Zeta.High.Thread.fst
@@ -5,7 +5,7 @@ let lemma_blum_add_elem_props (#app:_) (tl: verifiable_log app) (i: seq_index tl
                     let be = blum_add_elem tl i in
                     let gk,gv = be.r in
                     add_slot (index tl i) = to_base_key gk))
-  = admit()
+  = lemma_state_transition tl i
 
 let lemma_blum_evict_elem_key (#app:_) (tl: verifiable_log app) (i: seq_index tl {is_blum_evict tl i})
   : Lemma (ensures (let open Zeta.MultiSetHashDomain in
@@ -19,14 +19,126 @@ let lemma_blum_evict_elem_key (#app:_) (tl: verifiable_log app) (i: seq_index tl
                     gv = stored_value st_pre k /\
                     be.t = blum_evict_timestamp (index tl i) /\
                     be.tid = fst tl))
-  = admit()
+  = ()
 
-let not_refs_implies_store_unchanged  (#app:_) (k:Zeta.Key.base_key)
+#push-options "--z3rlimit_factor 3"
+
+let not_refs_implies_store_unchanged_addm  (#app:_) (ki:Zeta.Key.base_key)
+  (tl: verifiable_log app) (i:seq_index tl)
+  : Lemma (requires (let e = index tl i in
+                     let st_pre = store_pre tl i in
+                     let st_post = store_post tl i in
+                     AddM? (index tl i) /\
+                     not (e `exp_refs_key` ki) /\
+                     store_contains st_pre ki))
+          (ensures (let e = index tl i in
+                    let st_pre = store_pre tl i in
+                    let st_post = store_post tl i in
+                    store_contains st_post ki /\ st_pre ki == st_post ki))
+  = lemma_state_transition tl i
+
+let not_refs_implies_store_unchanged_addb  (#app:_) (ki:Zeta.Key.base_key)
+  (tl: verifiable_log app) (i:seq_index tl)
+  : Lemma (requires (let e = index tl i in
+                     let st_pre = store_pre tl i in
+                     let st_post = store_post tl i in
+                     AddB? (index tl i) /\
+                     not (e `exp_refs_key` ki) /\
+                     store_contains st_pre ki))
+          (ensures (let e = index tl i in
+                    let st_pre = store_pre tl i in
+                    let st_post = store_post tl i in
+                    store_contains st_post ki /\ st_pre ki == st_post ki))
+  = lemma_state_transition tl i
+
+let not_refs_implies_store_unchanged_evictm  (#app:_) (ki:Zeta.Key.base_key)
+  (tl: verifiable_log app) (i:seq_index tl)
+  : Lemma (requires (let e = index tl i in
+                     let st_pre = store_pre tl i in
+                     let st_post = store_post tl i in
+                     EvictM? (index tl i) /\
+                     not (e `exp_refs_key` ki) /\
+                     store_contains st_pre ki))
+          (ensures (let e = index tl i in
+                    let st_pre = store_pre tl i in
+                    let st_post = store_post tl i in
+                    store_contains st_post ki /\ st_pre ki == st_post ki))
+  = lemma_state_transition tl i
+
+let not_refs_implies_store_unchanged_evictb  (#app:_) (ki:Zeta.Key.base_key)
+  (tl: verifiable_log app) (i:seq_index tl)
+  : Lemma (requires (let e = index tl i in
+                     let st_pre = store_pre tl i in
+                     let st_post = store_post tl i in
+                     EvictB? (index tl i) /\
+                     not (e `exp_refs_key` ki) /\
+                     store_contains st_pre ki))
+          (ensures (let e = index tl i in
+                    let st_pre = store_pre tl i in
+                    let st_post = store_post tl i in
+                    store_contains st_post ki /\ st_pre ki == st_post ki))
+  = lemma_state_transition tl i
+
+let not_refs_implies_store_unchanged_evictbm  (#app:_) (ki:Zeta.Key.base_key)
+  (tl: verifiable_log app) (i:seq_index tl)
+  : Lemma (requires (let e = index tl i in
+                     let st_pre = store_pre tl i in
+                     let st_post = store_post tl i in
+                     EvictBM? (index tl i) /\
+                     not (e `exp_refs_key` ki) /\
+                     store_contains st_pre ki))
+          (ensures (let e = index tl i in
+                    let st_pre = store_pre tl i in
+                    let st_post = store_post tl i in
+                    store_contains st_post ki /\ st_pre ki == st_post ki))
+  = lemma_state_transition tl i
+
+let not_refs_implies_store_unchanged_runapp  (#app:_) (ki:Zeta.Key.base_key)
+  (tl: verifiable_log app) (i:seq_index tl)
+  : Lemma (requires (let e = index tl i in
+                     let st_pre = store_pre tl i in
+                     let st_post = store_post tl i in
+                     RunApp? (index tl i) /\
+                     not (e `exp_refs_key` ki) /\
+                     store_contains st_pre ki))
+          (ensures (let e = index tl i in
+                    let st_pre = store_pre tl i in
+                    let st_post = store_post tl i in
+                    store_contains st_post ki /\ st_pre ki == st_post ki))
+  = let e = index tl i in
+    let vs_pre = state_pre tl i in
+    let vs_post = state_post tl i in
+
+    lemma_state_transition tl i;
+    assert(vs_post == verify_step e vs_pre);
+
+    runapp_doesnot_change_nonref_slots e vs_pre ki;
+    assert((Some?.v (vs_pre.st ki)).r = (Some?.v (vs_post.st ki)).r);
+    runapp_doesnot_change_store_addmethod ki e vs_pre
+
+#pop-options
+
+let not_refs_implies_store_unchanged  (#app:_) (ki:Zeta.Key.base_key)
   (tl: verifiable_log app) (i:seq_index tl)
   : Lemma (ensures (let e = index tl i in
                     let st_pre = store_pre tl i in
                     let st_post = store_post tl i in
-                    not (e `exp_refs_key` k) ==>
-                    store_contains st_pre k ==>
-                    (store_contains st_post k /\ st_pre k == st_post k)))
-  = admit()
+                    not (e `exp_refs_key` ki) ==>
+                    store_contains st_pre ki ==>
+                    (store_contains st_post ki /\ st_pre ki == st_post ki)))
+  = let e = index tl i in
+    let vs_pre = state_pre tl i in
+    let vs_post = state_post tl i in
+
+    lemma_state_transition tl i;
+    assert(vs_post == verify_step e vs_pre);
+
+    if not (e `exp_refs_key` ki) && store_contains vs_pre.st ki then (
+      match e with
+      | RunApp _ _ _ -> not_refs_implies_store_unchanged_runapp ki tl i
+      | AddM _ _ _ -> not_refs_implies_store_unchanged_addm ki tl i
+      | AddB _ _ _ _ -> not_refs_implies_store_unchanged_addb ki tl i
+      | EvictM _ _ -> not_refs_implies_store_unchanged_evictm ki tl i
+      | EvictB _ _ -> not_refs_implies_store_unchanged_evictb ki tl i
+      | EvictBM _ _ _ -> not_refs_implies_store_unchanged_evictbm ki tl i
+      | _ -> ())
